wip on closed stuff

src/Closed.v
@@ -41,6 +41,7 @@ Fixpoint unroll_elim' (case : expr)
 Definition unroll_elim case ctor args mk_rec :=
     unroll_elim' case ctor args mk_rec 0.
 
+Module subst.
 Section subst.
 Open Scope option_monad.
 
@@ -61,6 +62,7 @@ Definition subst (arg : expr) (vals : list expr) (e : expr) : option expr :=
         end in
     go e.
 End subst.
+
 
 Inductive step : expr -> expr -> Prop :=
 | CloseStep : forall body vs e e' es,
@@ -92,6 +94,323 @@ Inductive step : expr -> expr -> Prop :=
     Forall value args ->
     step (Elim ty cases (Constr c args))
         (unroll_elim case c args (Elim ty cases)).
+
+Inductive star : expr -> expr -> Prop :=
+| StarNil : forall e, star e e
+| StarCons : forall e e' e'',
+        step e e' ->
+        star e' e'' ->
+        star e e''.
+
+Inductive plus : expr -> expr -> Prop :=
+| PlusOne : forall s s',
+        step s s' ->
+        plus s s'
+| PlusCons : forall s s' s'',
+        step s s' ->
+        plus s' s'' ->
+        plus s s''.
+
+Inductive initial_state (prog : list expr * list metadata) : expr -> Prop :=
+| initial_intro :
+    forall expr,
+      In expr (fst prog) ->
+      initial_state prog expr.
+
+Inductive final_state (prog : list expr * list metadata) : expr -> Prop :=
+| final_intro :
+    forall expr,
+      value expr ->
+      final_state prog expr.
+
+Definition semantics (prog : list expr * list metadata) : Semantics.semantics :=
+  @Semantics.Semantics_gen expr unit
+                 (fun _ => step)
+                 (initial_state prog)
+                 (final_state prog)
+                 tt.
+End subst.
+
+Module ksubst.
+
+Inductive cont :=
+| kStop : cont
+| kCloseArg (body : expr) (vs es : list expr) (k : cont)
+| kConstrArg (tag : constr_name) (vs es : list expr) (k : cont)
+| kCallL (r : expr) (k : cont)
+| kCallR (l : expr) (k : cont)
+| kElim (ty : type_name) (cases : list expr) (k : cont)
+.
+
+Fixpoint uncont (e : expr) (k : cont) : expr :=
+  match k with
+  | kStop => e
+  | kCloseArg body vs es k => Close body (vs ++ [uncont e k] ++ es)
+  | kConstrArg tag vs es k => Constr tag (vs ++ [uncont e k] ++ es)
+  | kCallL r k => Call (uncont e k) r
+  | kCallR l k => Call l (uncont e k)
+  | kElim ty cases k => Elim ty cases (uncont e k)
+  end.
+
+Inductive state :=
+| Run (e : expr) (k : cont)
+| Stop (e : expr)
+.
+
+Inductive kstep : state -> state -> Prop :=
+| KCloseStep : forall body vs e es k,
+        Forall value vs ->
+        ~ value e ->
+        kstep (Run (Close body (vs ++ [e] ++ es)) k)
+              (Run e (kCloseArg body vs es k))
+| KConstrStep : forall body vs e es k,
+        Forall value vs ->
+        ~ value e ->
+        kstep (Run (Constr body (vs ++ [e] ++ es)) k)
+              (Run e (kConstrArg body vs es k))
+
+| KCallL : forall e1 e2 k,
+        ~ value e1 ->
+        kstep (Run (Call e1 e2) k)
+              (Run e1 (kCallL e2 k))
+| KCallR : forall e1 e2 k,
+        value e1 ->
+        ~ value e2 ->
+        kstep (Run (Call e1 e2) k)
+              (Run e2 (kCallR e1 k))
+| KMakeCall : forall free arg k body e',
+        Forall value free ->
+        value arg ->
+        subst.subst arg free body = Some e' ->
+        kstep (Run (Call (Close body free) arg) k)
+              (Run e' k)
+
+| KElimStep : forall ty cases target k,
+        ~ value target ->
+        kstep (Run (Elim ty cases target) k)
+              (Run target (kElim ty cases k))
+| KEliminate : forall ty cases c args k case e',
+        is_ctor_for_type ty c ->
+        constructor_arg_n c = length args ->
+        nth_error cases (constructor_index c) = Some case ->
+        Forall value args ->
+        unroll_elim case c args (fun x => Elim ty cases x) = e' ->
+        kstep (Run (Elim ty cases (Constr c args)) k)
+              (Run e' k)
+
+| kContCloseArg : forall v body vs es k,
+    value v ->
+    kstep (Run v (kCloseArg body vs es k))
+          (Run (Close body (vs ++ [v] ++ es)) k)
+| kContConstrArg : forall v tag vs es k,
+    value v ->
+    kstep (Run v (kConstrArg tag vs es k))
+          (Run (Constr tag (vs ++ [v] ++ es)) k)
+| kContCallL : forall v r k,
+    value v ->
+    kstep (Run v (kCallL r k))
+          (Run (Call v r) k)
+| kContCallR : forall v l k,
+    value v ->
+    kstep (Run v (kCallR l k))
+          (Run (Call l v) k)
+| kContElim : forall v ty cases k,
+    value v ->
+    kstep (Run v (kElim ty cases k))
+          (Run (Elim ty cases v) k)
+| kContStop : forall v,
+    value v ->
+    kstep (Run v kStop)
+          (Stop v)
+.
+
+Inductive star : state -> state -> Prop :=
+| StarNil : forall e, star e e
+| StarCons : forall e e' e'',
+        kstep e e' ->
+        star e' e'' ->
+        star e e''.
+
+Inductive plus : state -> state -> Prop :=
+| PlusOne : forall s s',
+        kstep s s' ->
+        plus s s'
+| PlusCons : forall s s' s'',
+        kstep s s' ->
+        plus s' s'' ->
+        plus s s''.
+
+Inductive initial_state (prog : list expr * list metadata) : state -> Prop :=
+| initial_intro :
+    forall expr,
+      In expr (fst prog) ->
+      initial_state prog (Run expr kStop).
+
+Inductive final_state (prog : list expr * list metadata) : state -> Prop :=
+| final_intro :
+    forall expr,
+      value expr ->
+      final_state prog (Stop expr).
+
+Definition semantics (prog : list expr * list metadata) : Semantics.semantics :=
+  @Semantics.Semantics_gen state unit
+                 (fun _ => kstep)
+                 (initial_state prog)
+                 (final_state prog)
+                 tt.
+End ksubst.
+
+Module subst_equiv_ksubst.
+Import ksubst.
+Section subst_equiv_ksubst.
+  Variable prog : list expr * list metadata.
+
+  (*
+
+   Things to know about I.
+   * initial condition: forall e, I e (Run e kStop)
+   * final condition: value v -> I v s -> s = Stop v.
+   * simulation: I e s -> step e e' -> exists s', plus s s' /\ I e' s'
+   * refocusing: I e (Run h k) ->
+       can move enough of h into k to find "where the next step happens".
+   *)
+
+  Inductive I_expr : expr -> expr -> cont -> Prop :=
+  | IeCallL : forall e1 e2 h k,
+      ~ value e1 ->
+      I_expr e1 h k -> 
+      I_expr (Call e1 e2) h (kCallL e2 k)
+  | IeCallR : forall e1 e2 h k,
+      value e1 ->
+      ~ value e2 ->
+      I_expr e2 h k ->
+      I_expr (Call e1 e2) h (kCallR e1 k)
+  | IeMakeCall : forall body free e2,
+      Forall value free -> 
+      value e2 -> 
+      I_expr (Call (Close body free) e2) (Call (Close body free) e2) kStop
+  | IeConstrArg : forall tag vs e es h k,
+      Forall value vs ->
+      ~ value e ->
+      I_expr e h k ->
+      I_expr (Constr tag (vs ++ [e] ++ es)) h (kConstrArg tag vs es k)
+  | IeCloseArg : forall body vs e es h k,
+      Forall value vs ->
+      ~ value e ->
+      I_expr e h k ->
+      I_expr (Close body (vs ++ [e] ++ es)) h (kCloseArg body vs es k)
+  | IeElim : forall ty cases target h k,
+      ~ value target ->
+      I_expr target h k -> 
+      I_expr (Elim ty cases target) h (kElim ty cases k)
+  | IeEliminate : forall ty cases c args,
+      Forall value args -> 
+      I_expr (Elim ty cases (Constr c args)) (Elim ty cases (Constr c args)) kStop
+
+  | IeConstrDone : forall tag vs,
+      Forall value vs ->
+      I_expr (Constr tag vs) (Constr tag vs) kStop
+  | IeCloseDone : forall body vs,
+      Forall value vs ->
+      I_expr (Close body vs) (Close body vs) kStop
+  .
+  Hint Constructors I_expr.
+
+  Lemma value_no_step : 
+    forall e e', 
+      subst.step e e' -> 
+      value e -> 
+      False.
+  Proof.
+    induction 1; intro Hc; invc Hc.
+    - rewrite Forall_forall in *. intuition.
+    - rewrite Forall_forall in *. intuition.
+  Qed.
+  Hint Resolve value_no_step.
+
+  Lemma I_expr_uncont : 
+    forall e h k, I_expr e h k -> uncont h k = e.
+  Proof.
+    induction 1; simpl; auto using f_equal, f_equal2.
+  Qed.
+
+  Lemma I_expr_decompose : 
+    forall e e', subst.step e e' -> exists h k, I_expr e h k.
+  Proof.
+    induction 1; break_exists; eauto 10.
+  Qed.
+
+  Lemma I_expr_sim : 
+    forall e e', subst.step e e' -> forall h k, I_expr e h k -> exists h'
+
+  Inductive I : expr -> ksubst.state -> Prop := 
+  | IRun : forall e h k, I_expr e h k -> I e (Run h k)
+  | IStop : forall v, value v -> I v (Stop v).
+
+  Theorem I_sim :
+    forall e e',
+      subst.step e e' ->
+      forall s,
+        I e s ->
+        exists s', ksubst.plus s s' /\ I e' s'.
+  Proof.
+    intros.
+    invc H0; [| (* values don't step *) admit].
+    revert h k H1.
+    induction H; intros.
+    - 
+    
+    - 
+apply IeCloseArg in H1.
+invc H1.
+      + assert (vs0 = vs /\ e0 = e /\ es0 = es) by admit.
+        break_and. subst.
+        on (I _ _), fun H => apply IHstep in H.
+        break_exists_name s'. break_and.
+        eexists. split.
+        * eapply k
+      + (* values don't step *)
+
+  Lemma initial_states_match :
+    forall e,
+      initial_state (subst.semantics prog) e ->
+      exists s,
+        initial_state (semantics prog) s /\ I e s.
+  Proof.
+    simpl.
+    intros.
+    invc H.
+    eexists.
+    split.
+    - econstructor. eauto.
+    - econstructor.
+  Admitted.
+
+  Lemma match_final_state :
+    forall s s',
+      I s s' ->
+      final_state (subst.semantics prog) s ->
+      final_state (semantics prog) s'.
+  Proof.
+    simpl.
+    intros.
+    invc H0.
+    invc H.
+  Admitted.
+
+
+
+  Theorem fsim :
+    Semantics.forward_simulation (subst.semantics prog) (ksubst.semantics prog).
+  Proof.
+    eapply Semantics.forward_simulation_step.
+
+
+
+End subst_equiv_ksubst.
+End subst_equiv_ksubst.
+
+
 
 
 Inductive state :=
@@ -153,6 +472,8 @@ Inductive sstep : state -> state -> Prop :=
               (Run e' l k)
 .
 
+
+
 Inductive sstar : state -> state -> Prop :=
 | SStarNil : forall e, sstar e e
 | SStarCons : forall e e' e'',
@@ -187,3 +508,44 @@ Definition semantics (prog : list expr * list metadata) : Semantics.semantics :=
                  (initial_state prog)
                  (final_state prog)
                  tt.
+
+Module semantics_equiv.
+  Definition subst' l e :=
+    match l with
+    | [] => Some e
+    | arg :: free => subst.subst arg free e
+    end.
+
+(*
+Inductive I : expr -> state -> Prop :=
+| IRun_cons :
+    forall e1 e2 arg free k,
+      (forall v,
+          value v ->
+
+      I e1 (Run e2 l k)
+
+.
+*)
+
+Section preservation.
+  Variable prog : list expr * list metadata.
+
+
+  Lemma initial_states_match :
+    forall s,
+      Semantics.initial_state (subst.semantics prog) s ->
+      exists s',
+        Semantics.initial_state (semantics prog) s' /\ I s s'.
+  Proof.
+    intros.
+    invc H.
+    eexists.
+    split.
+    econstructor.
+    eauto.
+    simpl in s.
+
+
+  Theorem fsim : forward_simulation (subst.semantics prog) (semantics prog).
+  Proof.
